

<section permid="xyk" xml:id="s_background_formal-num-sys">
  <title>Formal Development of Number Systems</title>
  <introduction permid="GRW">
    <p permid="djU">
      Up to this point,
      we have been discussing number systems in an entirely informal manner,
      assuming everyone knew all that needed to be known.
      Now let's pause and put things on a more firm foundation.
      So for the time being,
      do a memory dump and forget everything you have ever learned about numbers and arithmetic.
      The set of natural numbers has just been delivered on our door step in a big box with a warning label saying <alert>Assembly Required.</alert> We open the box and find a single piece of paper on which the following
      <q>instructions</q> are printed.
      These defining properties of the natural numbers are known as the
      <term>Peano Postulates</term>.
          <idx><h>Peano postulates</h></idx>
      <ol permid="kez" label="i">
        <li permid="wsR">
          <p permid="ZFu">
            There is a non-empty set of elements called
            <term>natural numbers</term>.
              <idx><h>natural numbers</h></idx>
          There is natural number called <term>zero</term>
            which is denoted<nbsp /><m>0</m>.
            The set of all natural numbers is denoted <m>\nonnegints</m>
          </p>
        </li>

        <li permid="cAa">
          <p permid="FMD">
            There is a one-to-one function <m>s:\nonnegints \injection \nonnegints</m> called the
            <term>successor function</term>.
            For each <m>n\in \nonnegints</m>,
            <m>s(n)</m> is called the <term>successor</term>
              <idx><h>successor</h></idx>
            of <m>n</m>.
          </p>
        </li>

        <li permid="IHj">
          <p permid="lTM">
            There is no natural number <m>n</m> for which <m>0=s(n)</m>.
          </p>
        </li>

        <li permid="oOs" xml:id="peano_induction">

          <p permid="SaV">
            Let <m>\mathbb{M}\subseteq \nonnegints</m>.
            Then <m>\mathbb{M} =\nonnegints</m> if and only if

            <ol label="a">
              <li permid="DBR">
                <p permid="XuI">
                  <m>0\in \mathbb{M}</m>; and
                </p>
              </li>

              <li permid="UVB">
                <p permid="yie">
                  <m>\forall k\in \nonnegints\quad(k\in \mathbb{M}) 
                  \Longrightarrow(s(k)\in \mathbb{M})</m>.
                </p>
              </li>
            </ol>
          </p>
        </li>
      </ol>
    </p>

    <p permid="Jrd">
      Property <xref ref="peano_induction" /> in the list of Peano Postulates is called the
      <term>Principle of Mathematical Induction</term>,
      or just the <term>Principle of Induction</term>.
          <idx><h>induction</h><h>principle of mathematical</h></idx>
      As a first application of the Principle of Induction,
      we prove the following basic property of the natural numbers.
    </p>

    <proposition permid="aKN">
      <statement>
        <p permid="YAb">
          Let <m>n</m> be a natural number with <m>n\neq0</m>.
          Then there is a natural number <m>m</m> so that <m>n=s(m)</m>.
        </p>
      </statement>

      <proof permid="fuG">
        <p permid="CRX">
          Let <m>\mathbb{S}=\{n\in\nonnegints:\exists m\in\nonnegints,
          n=s(m)\}</m>.
          Then set <m>\mathbb{M}=\{0\}\cup\mathbb{S}</m>.
          We show that <m>\mathbb{M}=\nonnegints</m>.
          First, note that <m>0\in\mathbb{M}</m>.
          Next, we will show that for all <m>k\in\nonnegints</m>,
          if <m>k\in\mathbb{M}</m>, then <m>s(k)\in\mathbb{M}</m>.
          However, this is trivial since for all <m>k\in\nonnegints</m>,
          we have <m>s(k)\in\mathbb{S}\subseteq\mathbb{M}</m>.
          We conclude that <m>\mathbb{M}=\nonnegints</m>.
        </p>
      </proof>
    </proposition>
  </introduction>

  <subsection permid="dFt" xml:id="s_background_add">
    <title>Addition as a Binary Operation</title>
    <p permid="pym">
      A <term>binary operation</term>
          <idx><h>operation</h><h>binary</h></idx>
      <m>*</m> on set <m>X</m> is just a function <m>*:X\times X\rightarrow X</m>.
      So the image of the ordered pair <m>(x,y)</m> would normally be denoted <m>*((x,y))</m>.
      However, this is usually abbreviated as <m>*(x,y)</m> or even more compactly as <m>x*y</m>.
      With this convention,
      we now define a binary operation <m>+</m> on the set <m>\nonnegints</m> of natural numbers.
      This operation is defined as follows for every natural number <m>n\in\nonnegints</m>:

      <ol permid="QlI" label="i">
        <li permid="BcK">
          <p permid="epn">
            <m>n+0=n</m>.
          </p>
        </li>

        <li permid="hjT">
          <p permid="Kww">
            For all <m>k\in\nonnegints</m>, <m>n+s(k) = s(n+k)</m>.
          </p>
        </li>
      </ol>
    </p>

    <p permid="VFv">
      We pause to make it clear why the preceding two statements define <m>+</m>.
      Let <m>n</m> be an arbitrary natural number.
      Then let <m>\mathbb{M}</m> denote the set of all natural numbers <m>m</m> for which <m>n+m</m> is defined.
      Note that <m>0\in \mathbb{M}</m> by part<nbsp />(i).
      Also note that for all <m>k\in \nonnegints</m>,
      <m>s(k)\in \mathbb{M}</m> whenever <m>k\in \mathbb{M}</m> by part<nbsp />(ii).
      This shows that <m>\mathbb{M}=\nonnegints</m>.
      Since <m>n</m> was arbitrary,
      this allows us to conclude that <m>n+m</m> is defined for all <m>n,m\in \nonnegints</m>.
    </p>

    <p permid="BME">
      We read <m>n+m</m> as <m>n</m> <term>plus</term> <m>m</m>.
      The operation <m>+</m> is also called <term>addition</term>.
          <idx><h>addition</h><h>formal definition of</h></idx>
    </p>

    <p permid="hTN">
      Among the natural numbers, the successor of zero plays a very important role,
      so important that it deserves its own special symbol.
      Here we follow tradition and call the natural number <m>s(0)</m> <term>one</term>
      and denote it by<nbsp /><m>1</m>.
      Note that for every natural number <m>n</m>,
      we have <m>n+1=n+s(0)=s(n)</m>.
      In particular, <m>0+1=1</m>.
    </p>

    <p permid="OaW">
      With this notation,
      the Principle of Induction can be restated in the following form.
    </p>

    <principle permid="uDE">
      <title>Principle of Induction</title>
      <statement>
        <p permid="xcL">
          Let <m>\mathbb{M}\subseteq \nonnegints</m>.
          Then <m>\mathbb{M} =\nonnegints</m> if and only if

          <ol permid="DXq" label="a">
            <li permid="Nrc">
              <p permid="qDF">
                <m>0\in \mathbb{M}</m>; and
              </p>
            </li>

            <li permid="tyl">
              <p permid="WKO">
                <m>\forall k\in \nonnegints\quad(k\in \mathbb{M}) 
                \Longrightarrow(k+1\in \mathbb{M})</m>.
              </p>
            </li>
          </ol>
        </p>
      </statement>
    </principle>

    <theorem permid="JMC">
      <title>Associative Property of Addition</title>
      <statement>
        <p permid="geA">
          <m>m+(n+p) = (m+n)+p</m>, for all <m>m,n,p\in \nonnegints</m>.
        </p>
      </statement>

      <proof permid="mZf">
        <p permid="iZg">
          Let <m>m,n\in \nonnegints</m>.
          Then let <m>\mathbb{M}</m> denote the set of all natural numbers <m>p</m> for which <m>m+(n+p)=(m+n)+p</m>.
          We show that <m>\mathbb{M}=\nonnegints</m>.
        </p>

        <p permid="Pgp">
          Note that
          <me permid="Gwx">
            m+(n+0) = m+n = (m+n)+0
          </me>
          which shows that <m>0\in \mathbb{M}</m>.
        </p>

        <p permid="vny">
          Now assume that <m>k\in \mathbb{M}</m>,
          <ie />, <m>m+(n+k) = (m+n)+k</m>.
          Then
          <me permid="mDG">
            m+[n+(k+1)]=m+[(n+k)+1]=[m+(n+k)]+1= [(m+n)+k]+1=(m+n)+(k+1)
          </me>.
          Notice here that the first, second,
          and fourth equalities follow from the second part of the definition of addition while the third uses our inductive assumption that <m>m+(n+k)=(m+n)+k)</m>.
          This shows that <m>k+1\in \mathbb{M}</m>.
          Therefore, <m>\mathbb{M}= \nonnegints</m>.
          Since <m>m</m> and <m>n</m> were arbitrary elements of
          <m>\nonnegints</m>, the theorem follows.
        </p>
      </proof>
    </theorem>

    <p permid="uif">
      In proofs to follow,
      we will trim out some of the wording and leave only the essential mathematical steps intact.
      In particular,
      we will (i)<nbsp />omit reference to the set <m>\mathbb{M}</m>,
      and (ii)<nbsp />drop the phrase
      <q>For all <m>k\in\nonnegints</m></q>
      For example, to define addition,
      we will just write (i)<nbsp /><m>n+0=n</m>,
      and (ii)<nbsp /><m>n+(k+1) = (n+k)+1</m>.
    </p>

    <lemma permid="Cid">
      <statement>
        <p permid="EHk">
          <m>m+(n+1) = (m+1)+n</m>, for all <m>m,n\in\nonnegints</m>.
        </p>
      </statement>

      <proof permid="LBP">
        <p permid="buH">
          Fix <m>m\in \nonnegints</m>.
          Then
          <me permid="SKP">
            m+(0+1)=m+1= (m+0)+1
          </me>.
          Now assume that <m>m+(k+1)=(m+1)+k</m>.
          Then
          <me permid="yRY">
            m+[(k+1)+1]=[m+(k+1)]+1=[(m+1)+k]+1=(m+1)+(k+1)
          </me>.
        </p>
      </proof>
    </lemma>

    <p permid="apo">
      We next prove the commutative property,
      a task that takes two steps.
      First, we prove the following special case.
    </p>

    <lemma permid="ipm">
      <statement>
        <p permid="kOt">
          <m>n+0 = 0+n=n</m>, for all <m>n\in \nonnegints</m>.
        </p>
      </statement>

      <proof permid="rIY">
        <p permid="HBQ">
          The statement is trivially true when <m>n= 0</m>.
          Now suppose that <m>k+0=0+k=k</m> for some <m>k\in \nonnegints</m>.
          Then
          <me permid="eZh">
            (k+1) +0 = k+1 = (0+k)+1= 0+(k+1)
          </me>.
        </p>
      </proof>
    </lemma>

    <theorem permid="pTL">
      <title>Commutative Law of Addition</title>
      <statement>
        <p permid="MlJ">
          <m>m+n=n+m</m> for all <m>m,n\in \nonnegints</m>.
        </p>
      </statement>

      <proof permid="Tgo">
        <p permid="nIZ">
          Let <m>m\in \nonnegints</m>.
          Then <m>m+0=0+m</m> from the preceding lemma.
          Assume <m>m+k=k+m</m>.
          Then
          <me permid="Lgq">
            m+(k+1)=(m+k)+1=(k+m)+1= k+(m+1) = (k+1)+m
          </me>.
        </p>
      </proof>
    </theorem>

    <lemma permid="Owv" xml:id="lem_sum0">
      <statement>
        <p permid="QVC">
          If <m>m,n\in\nonnegints</m> and <m>m+n=0</m>, then <m>m=n=0</m>.
        </p>
      </statement>

      <proof permid="XQh">
        <p permid="TQi">
          Suppose that either of <m>m</m> and <m>n</m> is not zero.
          Since addition is commutative,
          we may assume without loss of generality that <m>n\neq0</m>.
          Then there exists a natural number <m>p</m> so that <m>n=s(p)</m>.
          This implies that <m>m+n=m+s(p)=s(m+p)=0</m>,
          which is impossible since <m>0</m> is not the successor of any natural number.
        </p>
      </proof>
    </lemma>

    <theorem permid="WaU">
      <title>Cancellation Law of Addition</title>
      <statement>
        <p permid="ssS">
          If <m>m,n,p\in \nonnegints</m> and <m>m+p=n+p</m>, then <m>m=n</m>.
        </p>
      </statement>

      <proof permid="znx">
        <p permid="zXr">
          Let <m>m,n\in \nonnegints</m>.
          Suppose that <m>m+0=n+0</m>.
          Then <m>m=n</m>.
          Now suppose that <m>m=n</m> whenever <m>m+k=n+k</m>.
          If <m>m+(k+1)=n+(k+1)</m>, then
          <me permid="rnz">
            s(m+k)=(m+k)+1=m+(k+1)=n+(k+1)=(n+k)+1=s(n+k)
          </me>.
          Since <m>s</m> is an
          injection, this implies <m>m+k=n+k</m>.
          Thus <m>m=n</m>.
        </p>
      </proof>
    </theorem>
  </subsection>

</section>

