

<section permid="lcO" xml:id="s_background_mult">
  <title>Multiplication as a Binary Operation</title>
  <p permid="AVG">
    We define a binary operation <m>\times</m>,
    called <term>multiplication</term>,
    on the set of natural numbers.
    When <m>m</m> and <m>n</m> are natural numbers,
    <m>m\times n</m> is also called the <term>product</term>
    of <m>m</m> and <m>n</m>,
    and it sometimes denoted <m>m*n</m> and even more compactly as <m>mn</m>.
    We will use this last convention in the material to follow.
    Let <m>n\in \nonnegints</m>.
    We define

    <ol permid="mSb" label="i">
      <li permid="SZk"><m>n0=0</m>, and</li>

      <li permid="zgt"><m>n(k+1)=nk +n</m>.</li>
    </ol>
  </p>

  <p permid="hcP">
    Note that <m>10=0</m> and <m>01=00+0=0</m>.
    Also, note that <m>11=10+1=0+1=1</m>.
    More generally, from<nbsp />(ii) and <xref ref="lem_sum0" />,
    we conclude that if <m>m,n\neq0</m>, then <m>mn\neq0</m>.
  </p>

  <theorem permid="RjX">
    <title>Left Distributive Law</title>
    <statement>
      <p permid="QeE">
        <m>m(n+p)=mn + mp</m>, for all <m>m,n,p\in \nonnegints</m>.
      </p>
    </statement>

    <proof permid="CaZ">
      <p permid="fnC">
        Let <m>m,n\in \nonnegints</m>.
        Then
        <me permid="trh">
          m(n+0)=mn = mn +0 = mn+ m0
        </me>.
        Now assume <m>m(n+k) = mn + mk</m>.
        Then
        <md permid="Zyq">
          <mrow>m[n+(k+1)] \amp = m[(n+k)+1]=m(n+k)+m</mrow>
          <mrow>\amp =(mn+mk)+m=mn+(mk+m)= mn+m(k+1)</mrow>
        </md>.
      </p>
    </proof>
  </theorem>

  <theorem permid="xrg">
    <title>Right Distributive Law</title>
    <statement>
      <p permid="wlN">
        <m>(m+n)p=mp + np</m>, for all <m>m,n,p\in \nonnegints</m>.
      </p>
    </statement>

    <proof permid="iii">
      <p permid="LuL">
        Let <m>m,n\in \nonnegints</m>.
        Then
        <me permid="FFz">
          (m+n)0 =0 = 0+0 = m0 + n0
        </me>.
        Now assume <m>(m+n)k = mk + nk</m>.
        Then
        <md permid="lMI">
          <mrow>(m+n)(k+1)\amp =(m+n)k+(m+n)= (mk+nk) +(m+n)</mrow>
          <mrow>\amp =(mk+m)+(nk+n)=m(k+1)+n(k+1)</mrow>
        </md>.
      </p>
    </proof>
  </theorem>

  <theorem permid="dyp">
    <title>Associative Law of Multiplication</title>
    <statement>
      <p permid="csW">
        <m>m(np) = (mn)p</m>, for all <m>m,n,p\in \nonnegints</m>.
      </p>
    </statement>

    <proof permid="Opr">
      <p permid="rBU">
        Let <m>m,n\in \nonnegints</m>.
        Then
        <me permid="RTR">
          m(n0)= m0 = 0 = (mn)0
        </me>.
        Now assume that <m>m(nk)=(mn)k</m>.
        Then
        <me permid="yba">
          m[n(k+1)]= m(nk + n)= m(nk) + mn =(mn)k + mn = (mn)(k+1)
        </me>.
      </p>
    </proof>
  </theorem>

  <p permid="NjY">
    The commutative law requires some preliminary work.
  </p>

  <lemma permid="pMH">
    <statement>
      <p permid="oHo">
        <m>n0= 0n=0</m>, for all <m>n\in \nonnegints</m>.
      </p>
    </statement>

    <proof permid="aDJ">
      <p permid="XJd">
        The lemma holds trivially when <m>n=0</m>.
        Assume <m>k0=
        0k=0</m>.
        Then
        <me permid="eij">
          (k+1)0 =0 = 0+0= 0k+0=0(k+1)
        </me>.
      </p>
    </proof>
  </lemma>

  <lemma permid="VTQ">
    <statement>
      <p permid="UOx">
        <m>n1 =1n=n</m>, for every <m>n\in \nonnegints</m>.
      </p>
    </statement>

    <proof permid="GKS">
      <p permid="DQm">
        <m>01=00+0=0 =10</m>.
        Assume
        <m>k1=1k=k</m>.
        Then
        <me permid="Kps">
          (k+1)1=k1+11=1k+1=1(k+1)
        </me>.
      </p>
    </proof>
  </lemma>

  <theorem permid="JFy">
    <title>Commutative Law of Multiplication</title>
    <statement>
      <p permid="IAf">
        <m>mn=nm</m>, for all <m>m,n\in \nonnegints</m>.
      </p>
    </statement>

    <proof permid="uwA">
      <p permid="jXv">
        Let <m>m\in \nonnegints</m>.
        Then <m>m0=0m</m>.
        Assume <m>mk=km</m>.
        Then
        <me permid="qwB">
          m (k+1) = mk +m = km+m= km +1m=(k+1)m
        </me>.
      </p>
    </proof>
  </theorem>
</section>

