

<section permid="NyG" xml:id="s_genfunction_binom-app">
  <title>An Application of the Binomial Theorem</title>
  <p permid="bCl">
    In this section,
    we see how <xref ref="thm_newton-binomial" text="title" /> can be used to derive another useful identity.
    We begin by establishing a different recursive formula for <m>P(p,k)</m> than was used in our definition of it.
  </p>

  <lemma permid="ZMY">
    <statement>
      <p permid="jgK">
        For each <m>k\ge0</m>,
        <m>P(p,k+1)=P(p,k)(p-k)</m>.
      </p>
    </statement>

    <proof permid="ypI">
      <p permid="KEa">
        When <m>k=0</m>, both sides evaluate to <m>p</m>.
        Now assume validity when
        <m>k=m</m> for some non-negative integer <m>m</m>.
        Then
        <md permid="AeV">
          <mrow>P(p,m+2)\amp =pP(p-1,m+1)</mrow>
          <mrow>\amp = p[P(p-1,m)(p-1-m)]</mrow>
          <mrow>\amp =[pP(p-1,m)](p-1-m)</mrow>
          <mrow>\amp =P(p,m+1)[p-(m+1)]</mrow>
        </md>.
      </p>
    </proof>
  </lemma>

  <p permid="HJu">
    Our goal in this section will be to invoke <xref ref="thm_newton-binomial" text="title" /> with the exponent <m>p=-1/2</m>.
    To do so in a meaningful manner,
    we need a simplified expression for <m>C(-1/2,k)</m>,
    which the next lemma provides.
  </p>

  <lemma permid="FUh" xml:id="l_newbinom">
    <statement>
      <p permid="PnT">
        For each <m>k\ge0</m>,
        <m>\displaystyle\binom{-1/2}{k}=(-1)^k\frac{\binom{2k}{k}}{2^{2k}}</m>.
      </p>
    </statement>

    <proof permid="ewR">
      <p permid="qLj">
        We proceed by induction on <m>k</m>.
        Both sides reduce to <m>1</m> when <m>k=0</m>.
        Now assume validity when <m>k=m</m> for some non-negative integer <m>m</m>.
        Then
        <md permid="gme">
          <mrow>\binom{-1/2}{m+1} \amp =\frac{P(-1/2,m+1)}{(m+1)!}
          =\frac{P(-1/2,m)(-1/2-m)}{(m+1)m!}</mrow>
          <mrow>\amp =\frac{-1/2-m}{m+1}\binom{-1/2}{m}
          =(-1)\frac{2m+1}{2(m+1)}(-1)^m\frac{\binom{2m}{m}}{2^{2m}}</mrow>
          <mrow>\amp =(-1)^{m+1}\frac{1}{2^{2m}}
          \frac{(2m+2)(2m+1)}{(2m+2)2(m+1)}\binom{2m}{m}=
          (-1)^{m+1}\frac{\binom{2m+2}{m+2}}{2^{2m+2}}</mrow>
        </md>.
      </p>
    </proof>
  </lemma>

  <theorem permid="tFP" xml:id="t_sqrt">
    <statement>
      <p permid="CZB">
        The function <m>f(x)=(1-4x)^{-1/2}</m> is the generating function of the sequence <m>\{\binom{2n}{n}:n\ge0\}</m>.
      </p>
    </statement>

    <proof permid="Siz">
      <p permid="WSs">
        By <xref ref="thm_newton-binomial" text="title" /> and <xref ref="l_newbinom"  />, we know that
        <md permid="Mtn">
          <mrow>(1-4x)^{-1/2}\amp =\sum_{n=0}^\infty\binom{-1/2}{n}(-4x)^n</mrow>
          <mrow>\amp =\sum_{n=0}^\infty(-1)^n2^{2n}\binom{-1/2}{n}x^n</mrow>
          <mrow>\amp =\sum_{n=0}^\infty \binom{2n}{n}x^n</mrow>
        </md>.
      </p>
    </proof>
  </theorem>

  <p permid="nQD">
    We will return to this generating function in <xref ref="s_recurrence_rubots" />,
    where it will play a role in a seemingly new counting problem that actually is a problem we've already studied in disguise.
  </p>

  <p permid="TXM">
    Now recalling <xref ref="prop_genfunction-product" /> about the coefficients in the product of two generating functions,
    we are able to deduce the following corollary of <xref ref="t_sqrt" /> by squaring the function <m>f(x) = (1-4x)^{-1/2}</m>.
  </p>

  <corollary permid="mbq">
    <statement>
      <p permid="vvc">
        For all <m>n\ge0</m>,
        <me permid="sAw">
          2^{2n}=\sum_{k=0}^n\binom{2k}{k}\binom{2n-2k}{n-k}
        </me>.
      </p>
    </statement>
  </corollary>
</section>

