

<section permid="mxc" xml:id="s_genfunction_gen-bin-thm">
  <title>Newton's Binomial Theorem</title>
  <p permid="vQO">
    In <xref ref="ch_strings"  />,
    we discussed the binomial theorem and saw that the following formula holds for all integers <m>p\ge1</m>:
    <me permid="MOZ">
      (1+x)^p =\sum_{n=0}^{p}\binom{p}{n} x^n
    </me>.
    You should quickly realize that this formula implies that the generating function for the number of <m>n</m>-element subsets of a <m>p</m>-element set is <m>(1+x)^p</m>.
    The topic of generating functions is what leads us to consider what happens if we encounter <m>(1+x)^p</m> as a generating function with <m>p</m> not a positive integer.
    It turns out that,
    by suitably extending the definition of the binomial coefficients to real numbers,
    we can also extend the binomial theorem in a manner originally discovered by Sir Isaac Newton.
  </p>

  <p permid="bXX">
    We've seen several expressions that can be used to calculate the binomial coefficients,
    but in order to extend <m>C(p,k)</m> to real values of <m>p</m>,
    we will utilize the form
    <me permid="sWi">
      \binom{p}{k}=\frac{P(p,k)}{k!}
    </me>,
    recalling that we've defined <m>P(p,k)</m> recursively as
    <m>P(p,0)=1</m> for all integers <m>p\geq 0</m> and
    <m>P(p,k)=p P(p-1,k-1)</m> when <m>p\geq k > 0</m>
    (<m>k</m> an integer).
    Notice here, however,
    that the expression for <m>P(p,k)</m> makes sense for any real number <m>p</m>,
    so long as <m>k</m> is a non-negative integer.
    We make this definition formal.
  </p>

  <definition permid="yLu">
    <statement>
      <p permid="jCw">
        For all real numbers <m>p</m> and nonnegative integers <m>k</m>,
        the number <m>P(p,k)</m> is defined by

        <ol permid="KZM">
          <li permid="rgV"><m>P(p,0)=1</m> for all real numbers <m>p</m> and</li>

          <li permid="Xoe">
            <m>P(p,k) = p P(p-1,k-1)</m> for all real numbers <m>p</m> and integers <m>k>0</m>.
          </li>
        </ol>
      </p>
    </statement>
  </definition>

  <p permid="Ifg">
    (Notice that this definition does not require <m>p\geq k</m> as we did with integers.)
  </p>

  <p permid="omp">
    We are now prepared to extend the definition of binomial coefficient so that <m>C(p,k)</m> is defined for all real <m>p</m> and nonnegative integer values of <m>k</m>.
    We do this as follows.
  </p>

  <definition permid="eSD">
    <statement>
      <p permid="PJF">
        For all real numbers <m>p</m> and nonnegative integers <m>k</m>,
        <me permid="Zdr">
          \binom{p}{k}=\frac{P(p,k)}{k!}
        </me>.

        <notation>
          <usage>\binom{p}{k}</usage>
          <description>generalized binomial coefficient</description>
        </notation>

            <idx><h>binomial coefficient</h><h>generalized</h></idx>
      </p>
    </statement>
  </definition>

  <p permid="Uty">
    Note that <m>P(p,k)=C(p,k)= 0</m> when <m>p</m> and <m>k</m> are integers with <m>0\le p\lt k</m>.
    On the other hand,
    we have interesting new concepts such as <m>P(-5,4)=(-5)(-6)(-7)(-8)</m> and
    <me permid="FkA">
      \binom{-7/2}{5}=\frac{(-7/2)(-9/2)(-11/2)(-13/2)(-15/2)}{5!}
    </me>.
  </p>

  <p permid="AAH">
    With this more general definition of binomial coefficients in hand,
    we're ready to state Newton's Binomial Theorem for all non-zero real numbers.
    The proof of this theorem can be found in most advanced calculus books.
  </p>

  <theorem permid="SEl" xml:id="thm_newton-binomial">
    <title>Newton's Binomial Theorem</title>
    <idx><h>binomial theorem</h><h>Newton's</h></idx>
    <statement>
      <p permid="Dvn">
        For all real <m>p</m> with <m>p\neq0</m>,
        <me permid="lrJ">
          (1+x)^p=\sum_{n=0}^\infty\binom{p}{n}x^n
        </me>.
      </p>
    </statement>
  </theorem>

  <p permid="gHQ">
    Note that the general form reduces to the original version of the binomial theorem when <m>p</m> is a positive integer.
  </p>
</section>

