<section xml:id="s_background_exp">
    <title>Exponentiation</title>
    <p>We now define a binary operation called <term>exponentiation</term> which is defined only on those ordered pairs <m>(m,n)</m> of natural numbers where not both are zero. The notation for exponentiation is non-standard. In books, it is written <m>m^n</m> while the notations <m>m**n</m>, <m>m\wedge n</m> and <m>\exp(m,n)</m> are used in-line. We will use the <m>m^n</m> notation for the most part.
    </p>

    <p>When <m>m=0</m>, we set <m>0^n=0</m> for all <m>n\in\nonnegints</m> with <m>n\neq0</m>. Now let <m>m\neq0</m>. We define <m>m^n</m> by (i)<nbsp /><m>m^0=1</m> and (ii)<nbsp /><m>m^{k+1}=mm^k</m>.
    </p>

    <theorem>
        <statement>
            <p>For all <m>m,n,p\in\nonnegints</m> with <m>m\neq0</m>, <m>m^{n+p}=m^n\,m^p</m>.
            </p>
        </statement>

        <proof>
            <p>Let <m>m,n\in\nonnegints</m> with <m>m\neq0</m>. Then <m>m^{n+0}=m^n=m^n\,1=m^n\,m^0</m>.  Now suppose that <m>m^{n+k}=m^n\,m^k</m>.  Then
            <me>
                m^{n+(k+1)}=m^{(n+k)+1}=m\,m^{n+k}
                = m(m^n\,m^k)=m^n(m\,m^k)=m^n\,m^{k+1}.
            </me>
            </p>
        </proof>
    </theorem>
    <theorem>
        <statement>
            <p>For all <m>m,n,p\in\nonnegints</m> with <m>m\neq0</m>, <m>(m^n)^p=m^{np}</m>.
            </p>
        </statement>

        <proof>
            <p>Let <m>m,n\in\nonnegints</m> with <m>m\neq0</m>. Then <m>(m^n)^0=1=m^0=m^{n0}</m>. Now suppose that <m>(m^n)^k=m^{nk}</m>.  Then
            <me>
                (m^n)^{k+1}=m^n(m^n)^k=m^n(m^{nk})=m^{n+nk}=m^{n(k+1)}.
            </me>
            </p>
        </proof>
    </theorem>
</section>
