<section xml:id="s_background_rationals">
    <title>Obtaining the Rationals from the Integers</title>
    <introduction>
        <p>We consider the set <m>\rats</m> of all ordered pairs in <m>\ints\times \ints</m> of the form <m>(x,y)</m> with <m>y\neq 0</m>. Elements of <m>\rats</m> are called <term>rational numbers</term><idx><h>rational numbers</h></idx>, or <term>fractions</term>. Define an equivalence relation, denoted <m>=</m>, on <m>\rats</m> by setting <m>(x,y)=(z,w)</m> if and only if <m>xw=yz</m>. Here we should point out that the symbol <m>=</m> can be used (and often is) to denote an equivalence relation. It is not constrained to mean <q>identically the same.</q>
        </p>

        <p>When <m>q=(x,y)</m> is a fraction, <m>x</m> is called the <term>numerator</term><idx><h>numerator</h></idx> and <m>y</m> is called the <term>denominator</term><idx><h>denominator</h></idx> of <m>q</m>.  Remember that the denominator of a fraction is never zero.
        </p>

        <p>
            Addition of fractions is defined by
        <me>
            (a,b)+(c,d) = (ad+bc,bd),
        </me>
            while multiplication is defined by
        <me>
            (a,b)(c,d) = (ac,bd).
        </me>
            As was the case with integers, it is important to pause and prove that both operations are well defined.
        </p>

        <theorem>
            <statement>
                <p>Let <m>x,y,z,w\in\rats</m>.  If <m>x=y</m> and <m>z=w</m>, then <m>x+z=y+w</m> and <m>xz=yw</m>.
                </p>
            </statement>
        </theorem>

        <p>Addition and multiplication are both associative and commutative.  Also, we have the distributive property.
        </p>

        <theorem>
            <statement>
                <p>
                    Let <m>x,y,z\in Q</m>. Then
                  <ol>
                    <li><p><m>x+y=y+x</m> and <m>xy=yx</m>.</p></li>
                    <li><p><m>x+(y+z) = (x+y)+z</m> and <m>x(yz)=(xy)z</m>.</p></li>
                    <li><p><m>x(y+z)=xy+xz</m>.</p></li>
                
                  </ol>
                </p>
            </statement>
        </theorem>

        <p>The additive inverse of a fraction <m>(a,b)</m> is just <m>(-a,b)</m>.  Using this, we define subtraction for fractions: <m>(a,b)-(c,d)=(a,b)+(-c,d)</m>.
        </p>

        <p>When <m>(a,b)</m> is a fraction, and <m>a\neq 0</m>, the fraction <m>(b,a)</m> is the <term>reciprocal</term><idx><h>reciprocal</h></idx> of <m>(a,b)</m>. The reciprocal is also called the <term>multiplicative inverse</term><idx><h>multiplicative inverse</h></idx>, and the reciprocal of <m>x</m> is denoted <m>x^{-1}</m>. When <m>y\neq0</m>, we can then define <term>division</term> by setting <m>x/y=xy^{-1}</m>, <ie />, <m>(a,b)/(c,d)=(ad, bc)</m>. Of course, division by zero is not defined, a fact that you probably already knew!
        </p>

        <p>As was the case for both <m>\nonnegints</m> and <m>\ints</m>, when <m>n</m> is a positive integer, and <m>0</m> is the zero in <m>\rats</m>, we define <m>0^n=0</m>. When <m>x=(a,b)</m> is a fraction with <m>x\neq0</m> and <m>n</m> is a non-negative integer, we define <m>x^n</m> inductively by (i)<nbsp /><m>x^0=1</m> and (ii)<nbsp /><m>x^{n+1}=xx^n</m>.
        </p>

        <theorem>
            <statement>
                <p>If <m>x\in\rats</m>, <m>x\neq0</m>, and <m>m,n\in\ints</m>, then <m>x^mx^n=x^{m+m}</m> and <m>(x^m)^n=x^{mn}</m>.
                </p>
            </statement>
        </theorem>

        <p>Many folks prefer an alternate notation for fractions in which the numerator is written directly over the denominator with a horizontal line between them, so <m>(2,5)</m> can also be written as <m>\frac{2}{5}</m>.
        </p>

        <p>Via the map <m>g(x) = (x,1)=\frac{x}{1}</m>, we again say that the integers are a <q>subset</q> of the rationals. As before, note that <m>g(x+y) = g(x)+g(y)</m>, <m>g(x-y)=g(x)-g(y)</m> and <m>g(xy)=g(x)g(y)</m>.
        </p>

        <p>In the third grade, you were probably told that <m>5 =\frac{5}{1}</m>, but by now you are realizing that this is not exactly true.  Similarly, if you had told your teacher that <m>\frac{3}{4}</m> and <m>\frac{6}{8}</m> weren't really the same and were only <q>equal</q> in the broader sense of an equivalence relation defined on a subset of the cartesian product of the integers, you probably would have been sent to the Principal's office.
        </p>

        <p>Try to imagine the trouble you would have gotten into had you insisted that the real meaning of <m>\frac{1}{2}</m> was
        <me>
            \frac{1}{2} =\langle(\langle(s(s(0)),s(0))\rangle,
            \langle(s(s(0)),0)\rangle)\rangle
        </me>
        We can also define a total order on <m>\rats</m>. To do this, we assume that <m>(a,b),(c,d)\in\rats</m> have <m>b,d>0</m>. (If <m>b\lt 0</m>, for example, we would replace it by <m>(a',b')=(-a,-b)</m>, which is in the same equivalence class as <m>(a,b)</m> and has <m>b'>0</m>.) Then we set <m>(a,b)\leq (c,d)</m> in <m>\rats</m> if <m>ad\leq bc</m> in <m>\ints</m>.
        </p>
    </introduction>


    <subsection>
        <title>Integer Exponents</title>
        <p>When <m>n</m> is a positive integer and <m>0</m> is the zero in <m>\rats</m>, we define <m>0^n=0</m>. When <m>x\in\rats</m>, <m>x\neq 0</m> and <m>n\in\nonnegints</m>, we define <m>x^n</m> inductively by<nbsp />(i)<nbsp /><m>x^0=1</m> and <m>x^{k+1}=xx^k</m>. When <m>n\in\ints</m> and <m>n\lt 0</m>, we set <m>x^n=1/x^{-n}</m>.
        </p>

        <theorem>
            <statement>
                <p>If <m>x\in\rats</m>, <m>x\neq0</m>, and <m>m,n\in\ints</m>, then <m>x^mx^n=x^{m+m}</m> and <m>(x^m)^n=x^{mn}</m>.
                </p>
            </statement>
        </theorem>
    </subsection>

</section>
