<?xml version="1.0" encoding="UTF-8"?>
<exercises xml:id="s_recurrence_PI" component="runestone-PI">
  <title>Peer Instruction Questions</title>
  <exercise label="recurrence_PI_linear">
    <statement>
      <p>Which of the following recurrence equations are linear?</p>
    </statement>
    <choices>
      <choice correct="yes">
        <statement>
          <p><m>f_{n} = f_{n-1}+f_{n-2}</m></p>
        </statement>
      </choice>
      <choice correct="yes">
        <statement>
          <p><m>r_{n+1} = r_n + (n+1)</m></p>
        </statement>
      </choice>
      <choice>
        <statement>
          <p><m>t_{n} = \displaystyle\sum_{k=0}^n t_k t_{n-k}</m></p>
        </statement>
      </choice>
      <choice correct="yes">
        <statement>
          <p><m>s_{n+3} = n^2 s_{n+1} - s_n + 2^n</m></p>
        </statement>
      </choice>
      <choice>
        <statement>
          <p>None of the above</p>
        </statement>
      </choice>
    </choices>
  </exercise>
  <exercise label="recurrence_PI_homogeneous">
    <statement>
      <p>Which of the following recurrence equations are homogeneous?</p>
    </statement>
    <choices>
      <choice correct="yes">
        <statement>
          <p><m>f_{n} = f_{n-1}+f_{n-2}</m></p>
        </statement>
      </choice>
      <choice>
        <statement>
          <p><m>r_{n+1} = r_n + (n+1)</m></p>
        </statement>
      </choice>
      <choice correct="yes">
        <statement>
          <p><m>t_{n+2} = 3t_{n+1}-t_{n}</m></p>
        </statement>
      </choice>
      <choice>
        <statement>
          <p><m>s_{n+3} = n^2 s_{n+1} - s_n + 2^n</m></p>
        </statement>
      </choice>
      <choice>
        <statement>
          <p>None of the above</p>
        </statement>
      </choice>
    </choices>
  </exercise>
  <exercise label="recurrence_PI_solve-deg-one">
    <statement>
      <p>Which of the following funtions satisfy the advancement operator
        equation
        <m>(A-3)f=0</m>?</p>
    </statement>
    <choices>
      <choice>
        <statement>
          <p><m>f(n) = (-3)^n</m></p>
        </statement>
      </choice>
      <choice>
        <statement>
          <p><m>f(n) = 3^n</m></p>
        </statement>
      </choice>
      <choice>
        <statement>
          <p><m>f(n) = 7\cdot(3^n)</m></p>
        </statement>
      </choice>
      <choice>
        <statement>
          <p>None of the above</p>
        </statement>
      </choice>
    </choices>
  </exercise>
  
</exercises>